theories/GenericTyping.v
@@ -278,7 +278,7 @@ Section GenericTyping.
       [ Γ ,, vass na A |- eta_expand f ≅ eta_expand g : B ] ->
       [ Γ |- f ≅ g : tProd na A B ] ;
     convtm_nat {Γ} :
-      [|-Γ] -> [Γ |- tNat ≅ tNat] ;
+      [|-Γ] -> [Γ |- tNat ≅ tNat : U] ;
     convtm_zero {Γ} :
       [|-Γ] -> [Γ |- tZero ≅ tZero : tNat] ;
     convtm_succ {Γ} {n n'} :
@@ -381,6 +381,8 @@ Section GenericTyping.
       [Γ |- t ⇒* t : A] ;
     redtm_trans {Γ A} :>
       Transitive (red_tm Γ A) ;
+    redtm_rtc {Γ A t t'} :
+      [Γ |- t ⇒* t' : A] -> reflTransClos (osred_tm Γ A) t t'
   }.
 
 End GenericTyping.
@@ -456,7 +458,7 @@ Class GenericTypingProperties `(ta : tag)
 }.
 
 #[export] Hint Resolve wfc_wft wfc_ty wfc_convty wfc_convtm wfc_redty wfc_redtm : gen_typing.
-#[export] Hint Resolve wfc_nil wfc_cons wft_wk wft_U wft_prod wft_nat ty_wk ty_var ty_prod ty_lam ty_app convty_wk convty_uni convty_prod convtm_wk convtm_prod convtm_eta convneu_wk convneu_var convneu_app ty_nat ty_zero  ty_succ ty_natElim convty_nat convtm_nat convtm_zero convtm_succ convtm_natElimZero convtm_natElimSucc convneu_natElim | 2 : gen_typing.
+#[export] Hint Resolve wfc_nil wfc_cons wft_wk wft_U wft_prod wft_nat ty_wk ty_var ty_prod ty_lam ty_app convty_wk convty_uni convty_prod convtm_wk convtm_prod convtm_eta convneu_wk convneu_var convneu_app ty_nat ty_zero  ty_succ ty_natElim convty_nat convtm_nat convtm_zero convtm_succ convtm_natElimZero convtm_natElimSucc convneu_natElim redty_ty_src redtm_ty_src| 2 : gen_typing.
 #[export] Hint Resolve wft_term convty_term convtm_convneu | 4 : gen_typing.
 #[export] Hint Resolve ty_conv ty_exp convty_exp convtm_exp convtm_conv convneu_conv redtm_conv | 6 : gen_typing.
 
