theories/LogicalRelation/Reduction.v
@@ -12,83 +12,165 @@ Set Printing Primitive Projection Parameters.
 
 Lemma redSubst {Γ A B l} :
   [Γ ||-<l> B] ->
-  [Γ |- A :⇒*: B] ->
+  [Γ |- A ⇒* B] ->
   ∑ (RA : [Γ ||-<l> A]), [Γ ||-<l> A ≅ B | RA].
 Proof.
   intros RB; revert A; pattern l, Γ, B, RB; apply LR_rect_TyUr; clear l Γ B RB; intros l Γ.
   - intros ? [] ? redA. unshelve eexists.
     + apply LRU_; econstructor; tea; etransitivity; tea.
+      constructor; tea; gen_typing.
     + now constructor.
   - intros B [t] A ?. unshelve eexists.
     + apply LRne_; exists t; tea; etransitivity; tea.
+      constructor; tea; gen_typing.
     + exists t; tea.
   - intros B [na dom cod] A ? ihdom ihcod; cbn in *; unshelve eexists.
     + apply LRPi'; unshelve eexists na dom cod _ _; tea; etransitivity; tea.
+      constructor; tea; gen_typing.
     + unshelve eexists na dom cod; tea; cbn.
       1,2: intros; apply LRTyEqRefl_.
   - intros B [red] A ?; unshelve eexists.
-    + apply LRNat_; constructor; now eapply redtywf_trans.
+    + apply LRNat_; constructor; tea; etransitivity; tea.
+      constructor; tea; gen_typing.
     + now constructor.
+Qed.
+
+
+Lemma redwfSubst {Γ A B l} :
+  [Γ ||-<l> B] ->
+  [Γ |- A :⇒*: B] ->
+  ∑ (RA : [Γ ||-<l> A]), [Γ ||-<l> A ≅ B | RA].
+Proof.
+  intros ? []; now eapply redSubst.
 Qed.
 
 Lemma redSubstTerm {Γ A t u l} (RA : [Γ ||-<l> A]) :
   [Γ ||-<l> u : A | RA] ->
-  [Γ |- t :⇒*: u : A ] ->
+  [Γ |- t ⇒* u : A ] ->
   [Γ ||-<l> t : A | RA] × [Γ ||-<l> t ≅ u : A | RA].
 Proof.
   revert t u; pattern l, Γ, A, RA; apply LR_rect_TyUr; clear l Γ A RA; intros l Γ.
   - intros ? h ?? ru' redtu; pose (ru := ru'); destruct ru' as [T].
     assert [Γ |- A ≅ U] by (destruct h; gen_typing).
-    assert (redtu' : [Γ |-[ ta ] t :⇒*: u]) by gen_typing.
+    assert [Γ |- t : U] by (eapply ty_conv; [gen_typing| now escape]).
+    assert (redtu' : [Γ |-[ ta ] t ⇒* u]) by gen_typing.
     destruct (redSubst (A:=t) (RedTyRecFwd h rel) redtu') as [rTyt0].
     pose proof (rTyt := RedTyRecBwd h rTyt0).
     unshelve refine (let rt : [LRU_ h | Γ ||- t : A]:= _ in _).
-    1: exists T; tea; etransitivity; gen_typing.
-    split; tea; exists rt ru rTyt; tea.
-    apply TyEqRecFwd; irrelevance.
+    + exists T; tea; constructor; destruct red; tea.
+      etransitivity; tea; eapply redtm_conv; tea; now escape.
+    + split; tea; exists rt ru rTyt; tea.
+      apply TyEqRecFwd; irrelevance.
   - intros ???? ru' ?; pose (ru := ru'); destruct ru' as [n].
-    assert [Γ |-[ ta ] t :⇒*: u : neRedTy.ty neA]. {
-      eapply redtmwf_conv; tea. 
+    assert [Γ |- A ≅ neRedTy.ty neA]. 1:{
       destruct neA; cbn in *.
       eapply convty_exp.
        2: apply redtywf_refl; gen_typing.
        2: apply convty_term; now apply convtm_convneu.
        gen_typing.
     }
+    assert [Γ |-[ ta ] t ⇒* u : neRedTy.ty neA] by (eapply redtm_conv; tea). 
+    assert [Γ |-[ ta ] t : neRedTy.ty neA] by (eapply ty_conv; tea; gen_typing). 
     unshelve refine (let rt : [LRne_ l neA | Γ ||- t : A] := _ in _).
-    1: exists n; tea; etransitivity; tea.
-    split; tea; exists n n; tea; etransitivity; tea. 
+    + exists n; tea; destruct red; constructor; tea; now etransitivity.
+    + split; tea; exists n n; tea; destruct red; constructor; tea; now etransitivity. 
   - intros ? ΠA ihdom ihcod ?? ru' ?; pose (ru := ru'); destruct ru' as [f].
-    assert [Γ |-[ ta ] t :⇒*: u : PiRedTyPack.prod ΠA].
-    1: {
-      eapply redtmwf_conv; tea. 
+    assert [Γ |- A ≅ PiRedTyPack.prod ΠA]. 1:{
       destruct ΠA as [??? []]. cbn in *.
       eapply convty_exp; tea.
       now apply redtywf_refl.
     }
+    assert [Γ |-[ ta ] t ⇒* u : PiRedTyPack.prod ΠA] by now eapply redtm_conv. 
+    assert [Γ |-[ ta ] t : PiRedTyPack.prod ΠA] by (eapply ty_conv; gen_typing).
     unshelve refine (let rt : [LRPi' ΠA | Γ ||- t : A] := _ in _).
-    1: exists f; tea; etransitivity; tea.
+    1: exists f; tea; constructor; destruct red; tea; etransitivity; tea.
     split; tea; exists rt ru; tea.
     intros; cbn. apply eq; tea.
     now apply LREqTermRefl_.
   - intros ? NA t ? Ru red; inversion Ru; subst.
-    assert [Γ |- t :⇒*: nf : tNat].
-    + eapply redtmwf_trans; tea.
-      eapply redtmwf_conv; tea.
-      destruct NA; gen_typing.
-    + split; econstructor; tea.
-      now eapply reflNatRedTmEq.
+    assert [Γ |- A ≅ tNat] by (destruct NA; gen_typing).
+    assert [Γ |- t :⇒*: nf : tNat]. 1:{
+      constructor. 2: gen_typing.
+      1: eapply ty_conv; gen_typing.
+      etransitivity. 2: gen_typing.
+      now eapply redtm_conv.
+    }
+    split; econstructor; tea.
+    now eapply reflNatRedTmEq.
+Qed.
+
+Lemma redwfSubstTerm {Γ A t u l} (RA : [Γ ||-<l> A]) :
+  [Γ ||-<l> u : A | RA] ->
+  [Γ |- t :⇒*: u : A ] ->
+  [Γ ||-<l> t : A | RA] × [Γ ||-<l> t ≅ u : A | RA].
+Proof.
+  intros ? []; now eapply redSubstTerm.
 Qed.
 
 Lemma redSubstTermOneStep {Γ t u A l} (RA : [Γ ||-<l> A]) :
-  [Γ |- t : A] ->
   [Γ |- t ⇒ u : A ] ->
   [Γ ||-<l> u : A | RA] ->
   [Γ ||-<l> t : A | RA] × [Γ ||-<l> t ≅ u : A | RA].
 Proof.
   intros; escape.
-  eapply redSubstTerm; tea; constructor; tea.
+  eapply redSubstTerm; tea.
   now eapply redtm_one_step. 
+Qed.
+
+
+Lemma redFwd {Γ l A B} : [Γ ||-<l> A] -> [Γ |- A :⇒*: B] -> whnf B -> [Γ ||-<l> B].
+Proof.
+  intros RA; revert B; pattern l, Γ, A, RA; apply LR_rect_TyUr; clear l Γ A RA.
+  - intros ??? [??? red] ? red' ?. 
+    eapply LRU_.  unshelve erewrite (redtywf_det _ _ _ _ _ _ red' red); tea.
+    1: constructor. econstructor; tea. eapply redtywf_refl; gen_typing.
+  - intros ??? [? red] ? red' ?.
+    eapply LRne_.
+    unshelve erewrite (redtywf_det _ _ _ _ _ _ red' red); tea.
+    1: now constructor.
+    econstructor; tea.
+    eapply redtywf_refl; gen_typing.
+  - intros ??? [??? red] ?? ? red' ?.
+    eapply LRPi'. 
+    unshelve erewrite (redtywf_det _ _ _ _ _ _ red' red); tea.
+    1: constructor.
+    econstructor; tea.
+    eapply redtywf_refl; gen_typing.
+  - intros ??? [red] ? red' ?.
+    eapply LRNat_.
+    unshelve erewrite (redtywf_det _ _ _ _ _ _ red' red); tea.
+    1: constructor.
+    econstructor; tea.
+    eapply redtywf_refl; gen_typing.
+Qed.
+
+Lemma redTmFwd {Γ l A t u} {RA : [Γ ||-<l> A]} : 
+  [Γ ||-<l> t : A | RA] -> [Γ |- t :⇒*: u : A] -> whnf u -> [Γ ||-<l> u : A | RA].
+Proof.
+  revert t u; pattern l,Γ,A,RA; apply LR_rect_TyUr; clear l Γ A RA.
+  - intros ?????? [? red] red' ?.
+    unshelve erewrite (redtmwf_det _ _ _ _ _ _ _ _ red' red); tea.
+    1: now eapply isType_whnf.
+    econstructor; tea.
+    1: eapply redtmwf_refl; gen_typing.
+    eapply RedTyRecBwd. eapply redFwd. 
+    2,3: gen_typing.
+    now eapply RedTyRecFwd.
+  - intros ??? ??? [? red] red' ?.
+    unshelve erewrite (redtmwf_det _ _ _ _ _ _ _ _ red' red); tea.
+    1: now constructor.
+    econstructor; tea.
+    eapply redtmwf_refl; gen_typing.
+  - intros ???????? [? red] red' ?.
+    unshelve erewrite (redtmwf_det _ _ _ _ _ _ _ _ red' red); tea.
+    1: now eapply isFun_whnf.
+    econstructor; tea.
+    eapply redtmwf_refl; gen_typing.
+  - intros ?????? Rt red' ?; inversion Rt; subst.
+    unshelve erewrite (redtmwf_det _ _ _ _ _ _ _ _ red' red); tea.
+    1: now eapply NatProp_whnf.
+    econstructor; tea.
+    eapply redtmwf_refl; gen_typing.
 Qed.
 
 End Reduction.
