theories/Substitution/Introductions/Nat.v
@@ -1,0 +1,662 @@
+From LogRel.AutoSubst Require Import core unscoped Ast Extra.
+From LogRel Require Import Utils BasicAst Notations Context NormalForms Weakening GenericTyping LogicalRelation DeclarativeTyping DeclarativeInstance Validity.
+From LogRel.LogicalRelation Require Import Induction Irrelevance Escape Reflexivity Weakening Neutral Transitivity Reduction Application Universe SimpleArr.
+From LogRel.Substitution Require Import Irrelevance Properties Conversion SingleSubst Reflexivity.
+From LogRel.Substitution.Introductions Require Import Universe Pi SimpleArr Var.
+
+Set Universe Polymorphism.
+
+Section Nat.
+Context `{GenericTypingProperties}.
+
+Set Printing Primitive Projection Parameters.
+
+
+Lemma natRed {Γ l} : [|- Γ] -> [Γ ||-<l> tNat].
+Proof. 
+  intros; eapply LRNat_; constructor; eapply redtywf_refl; gen_typing.
+Defined.
+
+Lemma natValid {Γ l} (VΓ : [||-v Γ]) : [Γ ||-v<l> tNat | VΓ].
+Proof.
+  unshelve econstructor; intros.
+  + now eapply natRed.
+  + cbn; constructor; eapply redtywf_refl; gen_typing.
+Defined.
+
+Lemma natconvValid {Γ l} (VΓ : [||-v Γ]) (VNat : [Γ ||-v<l> tNat | VΓ]) : 
+  [Γ ||-v<l> tNat ≅ tNat | VΓ | VNat].
+Proof.
+  constructor; intros.
+  enough [Δ ||-<l> tNat ≅ tNat | natRed wfΔ] by irrelevance.
+  constructor; cbn; eapply redtywf_refl; gen_typing.
+Qed.
+
+Lemma redUOne {Γ} : [|- Γ] -> [Γ ||-U<one> U].
+Proof.
+  intros ; econstructor; [easy| gen_typing|eapply redtywf_refl; gen_typing].
+Defined.
+
+Lemma natTermRed {Δ} (wfΔ : [|-Δ]) : [Δ ||-<one> tNat : U | LRU_ (redUOne wfΔ)].
+Proof.
+  econstructor.
+  + eapply redtmwf_refl; gen_typing.
+  + constructor.
+  + gen_typing.
+  + now eapply (natRed (l:= zero)).
+Defined.
+
+Lemma natTermValid {Γ} (VΓ : [||-v Γ]):  [Γ ||-v<one> tNat : U | VΓ | UValid VΓ].
+Proof.
+  constructor; intros.
+  - eapply natTermRed. 
+  - eexists (natTermRed wfΔ) (natTermRed wfΔ) (natRed wfΔ); cbn.
+    + gen_typing.
+    + now eapply (natRed (l:=zero)).
+    + constructor; eapply redtywf_refl; gen_typing.
+Qed.
+
+Lemma zeroRed {Γ l} {NN : [Γ ||-Nat tNat]} (wfΓ : [|- Γ]): [Γ ||-<l> tZero : _ | LRNat_ l NN].
+Proof.
+  exists tZero.
+  1,2: gen_typing.
+  constructor.
+Defined.
+
+Lemma zeroRedEq {Γ l} {NN : [Γ ||-Nat tNat]} (wfΓ : [|- Γ]): [Γ ||-<l> tZero ≅ tZero : _ | LRNat_ l NN].
+Proof.
+  exists tZero tZero.
+  1-3: gen_typing.
+  constructor.
+Defined.
+
+Lemma zeroValid {Γ l} (VΓ : [||-v Γ]): 
+  [Γ ||-v<l> tZero : tNat | VΓ | natValid VΓ].
+Proof.
+  constructor; intros; cbn; [unshelve eapply zeroRed| unshelve eapply zeroRedEq]; tea.
+Qed.
+
+Lemma succRed {Γ l n} {NN : [Γ ||-Nat tNat]} :
+  [Γ ||-<l> n : _ | LRNat_ l NN] ->
+  [Γ ||-<l> tSucc n : _ | LRNat_ l NN].
+Proof.
+  intros Rn; exists (tSucc n).
+  + eapply redtmwf_refl; eapply ty_succ; now escape.
+  + eapply convtm_succ; eapply escapeEqTerm; now eapply LREqTermRefl_.
+  + now constructor.
+Defined.
+
+Lemma succRedEq {Γ l n n'} {NN : [Γ ||-Nat tNat]} :
+  [Γ ||-<l> n : _ | LRNat_ l NN] ->
+  [Γ ||-<l> n' : _ | LRNat_ l NN] ->
+  [Γ ||-<l> n ≅ n' : _ | LRNat_ l NN] ->
+  [Γ ||-<l> tSucc n ≅ tSucc n' : _ | LRNat_ l NN].
+Proof.
+  intros ???; escape; exists (tSucc n) (tSucc n').
+  1,2: eapply redtmwf_refl; now eapply ty_succ.
+  + now eapply convtm_succ.
+  + now constructor.
+Defined.
+
+Lemma succRedInv {Γ l n} {NN : [Γ ||-Nat tNat]} :
+  [Γ ||-<l> tSucc n : _ | LRNat_ l NN] ->
+  [Γ ||-<l> n : _ | LRNat_ l NN].
+Proof.
+  intros RSn; inversion RSn; subst. 
+  unshelve epose proof (redtmwf_whnf red _). 1: constructor.
+  subst. inversion prop; subst; tea.
+  match goal with H : [ _ ||-NeNf _ : _] |- _ => destruct H; inv_whne end.
+Qed.
+
+Lemma succValid {Γ l n} (VΓ : [||-v Γ]) 
+  (Vn : [Γ ||-v<l> n : tNat | VΓ | natValid VΓ]) :
+  [Γ ||-v<l> tSucc n : tNat | VΓ | natValid VΓ].
+Proof.
+  constructor; intros; cbn.
+  - instValid Vσ ; now unshelve eapply succRed.
+  - instAllValid Vσ Vσ' Vσσ'; now unshelve eapply succRedEq.
+Qed.
+
+Lemma succcongValid {Γ l n n'} (VΓ : [||-v Γ]) 
+  (Vn : [Γ ||-v<l> n : tNat | VΓ | natValid VΓ])
+  (Vn' : [Γ ||-v<l> n' : tNat | VΓ | natValid VΓ])
+  (Veqn : [Γ ||-v<l> n ≅ n' : tNat | VΓ | natValid VΓ]) :
+  [Γ ||-v<l> tSucc n ≅ tSucc n' : tNat | VΓ | natValid VΓ].
+Proof.
+  constructor; intros; cbn; instValid Vσ; now unshelve eapply succRedEq.
+Qed.
+
+
+Lemma rtc_osredtm_redtm {Γ A x y} :
+  reflTransClos (osred_tm Γ A) x y ->
+  [Γ |- y : A] ->
+  [Γ |- x ⇒* y : A].
+Proof.
+  intros r ?; induction r.
+  + now eapply redtm_refl.
+  + intros. etransitivity.
+    2: now eapply IHr.
+    now eapply redtm_one_step.
+Qed.
+
+Lemma rtc_osredtm_redtmwf {Γ A x y} :
+  reflTransClos (osred_tm Γ A) x y ->
+  [Γ |- y : A] ->
+  [Γ |- x :⇒*: y : A].
+Proof.
+  intros reds yty.
+  pose proof (rtc_osredtm_redtm reds yty).
+  constructor; tea; gen_typing.
+Qed.
+
+Lemma osredtm_ty_src {Γ t u A} : [Γ |- t ⇒ u : A] -> [Γ |- t : A].
+Proof.
+  intros ?%redtm_one_step; gen_typing.
+Qed.
+
+
+Lemma red_natElimSubst {Γ l nN P hz hs n n'} :
+  [Γ ,, vass nN tNat |- P] ->
+  [Γ |- hz : P[tZero..]] ->
+  [Γ |- hs : elimSuccHypTy nN P] ->
+  [Γ |- n :⇒*: n' : tNat ] ->
+  forall (RN : [Γ ||-<l> tNat]),
+  [Γ ||-<l> n' : tNat | RN] ->
+  (forall t t',
+    [Γ ||-<l> t : tNat | RN] ->
+    [Γ ||-<l> t' : tNat | RN] ->
+    [Γ ||-<l> t ≅ t' : tNat | RN] ->
+    [Γ |- P[t..] ≅ P[t'..]]) -> 
+  [Γ |- tNatElim P hz hs n :⇒*: tNatElim P hz hs n' : P[n..]].
+Proof.
+  intros hp hhz hhs red rN rn' congP.
+  generalize (tmr_wf_red _ _ _ _ red).
+  destruct red as [_ _ r%redtm_rtc]. 
+  induction r as [|??? step reds ih] ; intros red; escape.
+  - eapply redtmwf_refl; gen_typing.
+  - unshelve epose (reds' := rtc_osredtm_redtm reds _); tea.
+    specialize (ih rn' reds').
+    assert [Γ |- P[z..] ≅ P[x..]]. 1:{
+      eapply congP; tea.
+      2: eapply LRTmEqSym.
+      all: now eapply redSubstTerm.
+    }
+    assert [Γ |- P[y..] ≅ P[x..]]. 1:{
+      etransitivity; tea.
+      eapply congP; tea.
+      all: now eapply redSubstTerm.
+    }
+    constructor.
+    + eapply ty_natElim; tea. now eapply osredtm_ty_src.
+    + eapply ty_conv; gen_typing.
+    + etransitivity.
+      1: eapply redtm_one_step; now eapply osredtm_natElim.
+      eapply redtm_conv; tea.
+      now eapply tmr_wf_red.
+Qed.
+
+Lemma arr_subst_eq {A B σ} : (arr A B)[σ] = arr A[σ] B[σ].
+Proof. now bsimpl. Qed.
+
+Lemma shift_up_eq {t σ} : t⟨↑⟩[up_term_term σ] = t[σ]⟨↑⟩.
+Proof. now bsimpl. Qed.
+
+Lemma up_single_subst {t σ u} : t[up_term_term σ][u..] = t[u .:  σ].
+Proof.  now bsimpl. Qed.
+
+Lemma up_liftSubst_eq {σ t u} : t[up_term_term σ][u]⇑ = t[u .: ↑ >> up_term_term σ].
+Proof.
+  bsimpl. eapply ext_term; intros [|n]; cbn.
+  1: reflexivity.
+  unfold funcomp; now rewrite  rinstInst'_term.
+Qed.
+
+Lemma elimSuccHypTy_subst {nN P} σ :
+  elimSuccHypTy nN P[up_term_term σ] = (elimSuccHypTy nN P)[σ].
+Proof.
+  unfold elimSuccHypTy.
+  cbn. rewrite shift_up_eq.
+  rewrite liftSubstComm. cbn. 
+  now rewrite up_liftSubst_eq.
+Qed.
+
+Lemma liftSubst_singleSubst_eq {t u v: term} : t[u]⇑[v..] = t[u[v..]..].
+Proof. now bsimpl. Qed.
+
+Definition natElim {Γ A} (P hz hs : term) {n} {NA : [Γ ||-Nat A]} (p : NatProp NA n) : term.
+Proof.
+  destruct p.
+  - exact hz.
+  - exact (tApp (tApp hs n) (tNatElim P hz hs n)).
+  - exact (tNatElim P hz hs ne).
+Defined.
+
+Section NatElimRed.
+  Context {Γ l nN P hs hz}
+    (wfΓ : [|- Γ])
+    (NN : [Γ ||-Nat tNat])
+    (RN := LRNat_ _ NN)
+    (tyP : [Γ,, vass nN tNat |- P])
+    (eqP : [Γ,, vass nN tNat |- P ≅ P])
+    (RPpt : forall n, [Γ ||-<l> n : _ | RN] -> [Γ ||-<l> P[n..]])
+    (RPext : forall n n' (Rn : [Γ ||-<l> n : _ | RN]),
+      [Γ ||-<l> n' : _ | RN] ->
+      [Γ ||-<l> n ≅ n' : _ | RN] ->
+      [Γ ||-<l> P[n..] ≅ P[n'..] | RPpt _ Rn])
+    (RPz := RPpt _ (zeroRed wfΓ))
+    (Rhz : [Γ ||-<l> hz : P[tZero..] | RPz]) 
+    (RPs : [Γ ||-<l> elimSuccHypTy nN P])
+    (Rhs : [Γ ||-<l> hs : _ | RPs]).
+
+  Definition natRedElimStmt :=
+    (forall n (Rn : [Γ ||-<l> n : _ | RN]), 
+      [Γ ||-<l> tNatElim P hz hs n : _ | RPpt _ Rn ] ×
+      [Γ ||-<l> tNatElim P hz hs n ≅ tNatElim P hz hs (NatRedTm.nf Rn) : _ | RPpt _ Rn]) ×
+    (forall n (Nn : NatProp NN n) (Rn : [Γ ||-<l> n : _ | RN]), 
+      [Γ ||-<l> tNatElim P hz hs n : _ | RPpt _ Rn ] ×
+      [Γ ||-<l> tNatElim P hz hs n ≅ natElim P hz hs Nn : _ | RPpt _ Rn]).
+
+  Lemma natElimRedAux : natRedElimStmt.
+  Proof.
+    escape.
+    apply NatRedInduction.
+    - intros ? nf red ? nfprop ih.
+      assert [Γ ||-<l> nf : _ | RN]. 1:{
+        econstructor; tea.
+        eapply redtmwf_refl; gen_typing.
+      }
+      eapply redwfSubstTerm.
+      + eapply LRTmRedConv. 
+        2: unshelve eapply ih; tea.
+        eapply RPext. 
+        2: eapply LRTmEqSym.
+        1,2: eapply redwfSubstTerm; tea.
+      + eapply red_natElimSubst; tea.
+        intros; eapply escapeEq; now eapply RPext.
+    - intros. 
+      eapply redSubstTermOneStep.
+      1: eapply osredtm_natElimZero; tea.
+      irrelevance.
+    - intros n Rn ih RSucc; change [Γ ||-<l> n : tNat | RN] in Rn.
+      eapply redSubstTermOneStep.
+      1: eapply osredtm_natElimSucc; tea.
+      1: now escape.
+      eapply simple_appTerm.
+      2: eapply ih.
+      irrelevance0.
+      2: unshelve eapply (appTerm RPs Rhs Rn).
+      now bsimpl.
+    - intros ? [] ?.
+      eapply neuTerm_aux; cbn.
+      1,2: now constructor.
+      1,2: now eapply ty_natElim.
+      eapply convneu_natElim; tea.
+      all: eapply escapeEqTerm; now eapply LREqTermRefl_.
+    Unshelve.
+    * tea.
+    * eapply ArrRedTy; now eapply RPpt.
+    * rewrite arr_subst_eq. eapply ArrRedTy.
+      2: rewrite liftSubst_singleSubst_eq; cbn.
+      all: now eapply RPpt.
+  Qed.
+  
+  Lemma natElimRed : forall n (Rn : [Γ ||-<l> n : _ | RN]), [Γ ||-<l> tNatElim P hz hs n : _ | RPpt _ Rn ].
+  Proof. intros. apply (fst natElimRedAux). Qed.
+End NatElimRed.
+
+
+Section NatElimRedEq.
+  Context {Γ l nN P Q hs hs' hz hz'}
+    (wfΓ : [|- Γ])
+    (NN : [Γ ||-Nat tNat])
+    (RN := LRNat_ _ NN)
+    (tyP : [Γ,, vass nN tNat |- P])
+    (tyQ : [Γ,, vass nN tNat |- Q])
+    (eqPQ : [Γ,, vass nN tNat |- P ≅ Q])
+    (RPpt : forall n, [Γ ||-<l> n : _ | RN] -> [Γ ||-<l> P[n..]])
+    (RQpt : forall n, [Γ ||-<l> n : _ | RN] -> [Γ ||-<l> Q[n..]])
+    (RPQext : forall n n' (Rn : [Γ ||-<l> n : _ | RN]),
+      [Γ ||-<l> n' : _ | RN] ->
+      [Γ ||-<l> n ≅ n' : _ | RN] ->
+      [Γ ||-<l> P[n..] ≅ Q[n'..] | RPpt _ Rn])
+    (RPz := RPpt _ (zeroRed wfΓ))
+    (RQz := RQpt _ (zeroRed wfΓ))
+    (Rhz : [Γ ||-<l> hz : P[tZero..] | RPz]) 
+    (RQhz : [Γ ||-<l> hz' : Q[tZero..] | RQz]) 
+    (RPQhz : [Γ ||-<l> hz ≅ hz' : _ | RPz])
+    (RPs : [Γ ||-<l> elimSuccHypTy nN P])
+    (RQs : [Γ ||-<l> elimSuccHypTy nN Q])
+    (Rhs : [Γ ||-<l> hs : _ | RPs])
+    (RQhs : [Γ ||-<l> hs' : _ | RQs])
+    (RPQhs : [Γ ||-<l> hs ≅ hs' : _ | RPs ])
+    .
+
+  Lemma RPext : forall n n' (Rn : [Γ ||-<l> n : _ | RN]),
+      [Γ ||-<l> n' : _ | RN] ->
+      [Γ ||-<l> n ≅ n' : _ | RN] ->
+      [Γ ||-<l> P[n..] ≅ P[n'..] | RPpt _ Rn].
+  Proof.
+    intros. eapply transEq; [| eapply LRTyEqSym ]; eapply RPQext; cycle 1; tea.
+    now eapply LREqTermRefl_.
+    Unshelve. 3,4: eauto. tea.
+  Qed.
+
+  Lemma natElimRedAuxLeft : @natRedElimStmt _ _ P hs hz NN RPpt.
+  Proof.
+    eapply natElimRedAux; tea.
+    + now eapply lrefl.
+    + eapply RPext.
+  Qed.
+
+  Lemma natElimRedAuxRight : @natRedElimStmt _ _ Q hs' hz' NN RQpt.
+  Proof.
+    eapply natElimRedAux; tea.
+    + now eapply urefl.
+    + intros. eapply transEq; [eapply LRTyEqSym |]; eapply RPQext; cycle 1; tea.
+      now eapply LREqTermRefl_.
+    Unshelve. 2: eauto. all:tea.
+  Qed.
+
+  Lemma natElimRedEqAux :
+    (forall n n' (Rnn' : [Γ ||-<l> n ≅ n' : _ | RN]) (Rn : [Γ ||-<l> n : _ | RN]) (Rn' : [Γ ||-<l> n' : _ | RN]), 
+      [Γ ||-<l> tNatElim P hz hs n ≅ tNatElim Q hz' hs' n' : _ | RPpt _ Rn ]) ×
+    (forall n n' (Rnn' : NatPropEq NN n n') (Rn : [Γ ||-<l> n : _ | RN]) (Rn' : [Γ ||-<l> n' : _ | RN]), 
+      [Γ ||-<l> tNatElim P hz hs n ≅ tNatElim Q hz' hs' n' : _ | RPpt _ Rn ]).
+  Proof.
+    apply NatRedEqInduction.
+    - intros ?? nfL nfR redL redR ? prop ih RL RR; destruct (NatPropEq_whnf prop).
+      assert [Γ ||-<l> nfL : _ | RN] by (eapply redTmFwd; cycle 1; tea).
+      assert [Γ ||-<l> nfR : _ | RN] by (eapply redTmFwd; cycle 1; tea).
+      eapply LREqTermHelper.
+      * eapply (fst natElimRedAuxLeft).
+      * eapply (fst natElimRedAuxRight).
+      * eapply RPQext. 1: tea.
+        now econstructor.
+      * eapply LRTmEqRedConv.
+        + eapply RPext; tea. 
+          eapply LRTmEqSym; eapply redwfSubstTerm; cycle 1; tea.
+        + unshelve erewrite (redtmwf_det _ _ _ _ _ _ _ _ (NatRedTm.red RL) redL); tea.
+          1: dependent inversion RL; subst; cbn; now eapply NatProp_whnf.
+          unshelve erewrite (redtmwf_det _ _ _ _ _ _ _ _ (NatRedTm.red RR) redR); tea.
+          1: dependent inversion RR; subst; cbn; now eapply NatProp_whnf.
+          now eapply ih.
+        Unshelve. tea.
+    - intros. eapply LREqTermHelper.
+      * unshelve eapply (snd natElimRedAuxLeft); constructor.
+      * unshelve eapply (snd natElimRedAuxRight); tea; constructor.
+      * eapply RPQext; [unshelve eapply zeroRed| unshelve eapply zeroRedEq]; tea.
+      * cbn; irrelevance.
+    - intros ??? ih Rn Rn'. pose proof (succRedInv Rn); pose proof (succRedInv Rn').
+      eapply LREqTermHelper.
+      * unshelve eapply (snd natElimRedAuxLeft); now constructor.
+      * unshelve eapply (snd natElimRedAuxRight); tea; now constructor.
+      * eapply RPQext; [unshelve eapply succRed| unshelve eapply succRedEq]; tea.
+      * cbn.
+        eapply simple_appcongTerm.
+        4: now eapply ih.
+        + irrelevance0. 2: eapply appcongTerm; tea.
+          now bsimpl.
+        + eapply (fst natElimRedAuxLeft).
+        + eapply LRTmRedConv. 2: eapply (fst natElimRedAuxRight).
+          eapply LRTyEqSym; now eapply RPQext.
+        Unshelve. 2,4,5: tea.
+        1: eapply ArrRedTy; now eapply RPpt.
+        rewrite arr_subst_eq. eapply ArrRedTy.
+        2: rewrite liftSubst_singleSubst_eq; cbn.
+        all: now eapply RPpt.
+    - intros ?? neueq ??. escape. inversion neueq.
+      assert [Γ |- P[ne..] ≅ Q[ne'..]]. 1:{
+        eapply escapeEq. eapply RPQext; tea.
+        econstructor.
+        1,2: now eapply redtmwf_refl.
+        2: now constructor.
+        gen_typing.
+      }
+      eapply neuTermEq.
+      1,2: now constructor.
+      * eapply ty_natElim; tea.
+      * eapply ty_conv. 
+        1: eapply ty_natElim; tea.
+        now symmetry.
+      * eapply convneu_natElim ; tea.
+      Unshelve. tea.
+  Qed.
+
+  Lemma natElimRedEq :
+    (forall n n' (Rnn' : [Γ ||-<l> n ≅ n' : _ | RN]) (Rn : [Γ ||-<l> n : _ | RN]) (Rn' : [Γ ||-<l> n' : _ | RN]), 
+      [Γ ||-<l> tNatElim P hz hs n ≅ tNatElim Q hz' hs' n' : _ | RPpt _ Rn ]).
+  Proof. apply natElimRedEqAux. Qed.
+End NatElimRedEq.
+
+
+
+Section NatElimValid.
+  Context {Γ l nN P}
+    (VΓ : [||-v Γ])
+    (VN := natValid (l:=l) VΓ)
+    (VΓN := validSnoc nN VΓ VN)
+    (VP : [Γ ,, vass nN tNat ||-v<l> P | VΓN]).
+  
+  Lemma elimSuccHypTyValid :
+    [Γ ||-v<l> elimSuccHypTy nN P | VΓ].
+  Proof.
+    unfold elimSuccHypTy.
+    unshelve eapply PiValid.
+    1: exact VN.
+    eapply simpleArrValid; tea.
+    eapply substLiftS; tea.
+    eapply irrelevanceTm.
+    eapply succValid.
+    eapply irrelevanceTm.
+    change tNat with tNat⟨@wk1 Γ nN tNat⟩ at 2.
+    eapply var0Valid.
+    Unshelve. all: tea.
+  Qed.
+
+  Context {hz hs}
+    (VPz := substS nN VP (zeroValid VΓ))
+    (Vhz : [Γ ||-v<l> hz : P[tZero..] | VΓ | VPz]) 
+    (Vhs : [Γ ||-v<l> hs : _ | VΓ | elimSuccHypTyValid]).
+
+
+  Lemma natElimValid {n}
+    (Vn : [Γ ||-v<l> n : tNat | VΓ | VN])
+    (VPn := substS nN VP Vn)
+    : [Γ ||-v<l> tNatElim P hz hs n : _ | VΓ | VPn].
+  Proof.
+    constructor; intros.
+    - instValid Vσ; cbn.
+      irrelevance0.  1: now rewrite singleSubstComm'.
+      epose proof (Vuσ := liftSubstS' nN VN Vσ).
+      instValid Vuσ; escape.
+      unshelve eapply natElimRed; tea.
+      + intros m Rm.
+        rewrite up_single_subst. 
+        unshelve eapply validTy; cycle 1; tea.
+        unshelve econstructor; [now bsimpl| now cbn].
+      + rewrite elimSuccHypTy_subst. eapply validTy; tea; eapply elimSuccHypTyValid.
+      + eapply escapeEq; eapply validTyEq; eapply reflValidTy.
+      + intros m m' Rm Rm' Rmm'; cbn.
+        irrelevance0. 1: now rewrite up_single_subst.
+        rewrite up_single_subst.
+        unshelve eapply validTyExt; cycle 1 ; tea.
+        1,2: unshelve econstructor; [now bsimpl| now cbn].
+        unshelve econstructor; [|now cbn].
+        bsimpl; cbn; eapply reflSubst.
+      + irrelevance.
+      + irrelevance. now rewrite elimSuccHypTy_subst. 
+    - instAllValid Vσ Vσ' Vσσ'.
+      irrelevance0.  1: now rewrite singleSubstComm'.
+      pose (Vuσ := liftSubstS' nN VN Vσ).
+      pose proof (Vuσ' := liftSubstS' nN VN Vσ').
+      pose proof (Vuσrea :=  liftSubstSrealign' nN VN Vσσ' Vσ').
+      pose proof (Vuσσ' := liftSubstSEq' nN VN Vσσ').
+      instValid Vuσ'; instAllValid Vuσ Vuσrea Vuσσ'; escape.
+      unshelve eapply natElimRedEq; tea; fold subst_term.
+      6-11: irrelevance; now rewrite elimSuccHypTy_subst.
+      3,4: rewrite elimSuccHypTy_subst; eapply validTy; tea; eapply elimSuccHypTyValid.
+      + intros m Rm.
+        rewrite up_single_subst. 
+        unshelve eapply validTy; cycle 1; tea.
+        unshelve econstructor; [now bsimpl| now cbn].
+      + intros m Rm.
+        rewrite up_single_subst. 
+        unshelve eapply validTy; cycle 1; tea.
+        unshelve econstructor; [now bsimpl| now cbn].
+      + intros m m' Rm Rm' Rmm'; cbn.
+        irrelevance0. 1: now rewrite up_single_subst.
+        rewrite up_single_subst.
+        unshelve eapply validTyExt; cycle 1 ; tea.
+        1,2: unshelve econstructor; [now bsimpl| now cbn].
+        unshelve econstructor; [|now cbn].
+        now bsimpl.
+      Unshelve. 4: tea. 1: gen_typing. 
+      now eapply irrelevanceSubst.
+  Qed. 
+
+  Lemma natElimZeroValid  : 
+    [Γ ||-v<l> tNatElim P hz hs tZero ≅ hz : _ | VΓ | VPz].
+  Proof.
+    constructor; intros.
+    epose proof (Vuσ := liftSubstS' nN VN Vσ).
+    instValid Vσ; instValid Vuσ; escape.
+    irrelevance0.  1: now rewrite singleSubstComm'.
+    unshelve eapply (snd (natElimRedAux _ _ _ _ _ _ _ _ _) _ NatRedTm.zeroR); tea; fold subst_term.
+    8: eapply zeroValid.
+    + eapply escapeEq; eapply validTyEq; eapply reflValidTy.
+    + intros m Rm.
+      rewrite up_single_subst. 
+      unshelve eapply validTy; cycle 1; tea.
+      unshelve econstructor; [now bsimpl| now cbn].
+    + intros m m' Rm Rm' Rmm'; cbn.
+      irrelevance0. 1: now rewrite up_single_subst.
+      rewrite up_single_subst.
+      unshelve eapply validTyExt; cycle 1 ; tea.
+      1,2: unshelve econstructor; [now bsimpl| now cbn].
+      unshelve econstructor; [|now cbn].
+      bsimpl; cbn; eapply reflSubst.
+    + irrelevance.
+    + rewrite elimSuccHypTy_subst. eapply validTy; tea; eapply elimSuccHypTyValid.
+    + irrelevance. now rewrite elimSuccHypTy_subst. 
+    Unshelve. 10: tea. 6: tea. 4: tea.
+  Qed.
+  
+  Lemma natElimSuccValid {n}
+    (Vn : [Γ ||-v<l> n : tNat | VΓ | VN]) 
+    (VPSn := substS nN VP (succValid _ Vn)) : 
+    [Γ ||-v<l> tNatElim P hz hs (tSucc n) ≅ tApp (tApp hs n) (tNatElim P hz hs n) : _ | VΓ | VPSn].
+  Proof.
+    constructor; intros.
+    epose proof (Vuσ := liftSubstS' nN VN Vσ).
+    instValid Vσ; instValid Vuσ; escape.
+    irrelevance0.  1: now rewrite singleSubstComm'.
+    pose (NSn := NatRedTm.succR RVn).
+    unshelve eapply (snd (natElimRedAux _ _ _ _ _ _ _ _ _) _ NSn); tea; fold subst_term.
+    + eapply escapeEq; eapply validTyEq; eapply reflValidTy.
+    + intros m Rm.
+      rewrite up_single_subst. 
+      unshelve eapply validTy; cycle 1; tea.
+      unshelve econstructor; [now bsimpl| now cbn].
+    + intros m m' Rm Rm' Rmm'; cbn.
+      irrelevance0. 1: now rewrite up_single_subst.
+      rewrite up_single_subst.
+      unshelve eapply validTyExt; cycle 1 ; tea.
+      1,2: unshelve econstructor; [now bsimpl| now cbn].
+      unshelve econstructor; [|now cbn].
+      bsimpl; cbn; eapply reflSubst.
+    + irrelevance.
+    + rewrite elimSuccHypTy_subst. eapply validTy; tea; eapply elimSuccHypTyValid.
+    + irrelevance. now rewrite elimSuccHypTy_subst. 
+    + now eapply succRed.
+    Unshelve. 4-6: tea.
+  Qed.
+
+End NatElimValid.
+
+Lemma natElimCongValid {Γ l nN P Q hz hz' hs hs' n n'}
+    (VΓ : [||-v Γ])
+    (VN := natValid (l:=l) VΓ)
+    (VΓN := validSnoc nN VΓ VN)
+    (VP : [Γ ,, vass nN tNat ||-v<l> P | VΓN])
+    (VQ : [Γ ,, vass nN tNat ||-v<l> Q | VΓN])
+    (VPQ : [Γ ,, vass nN tNat ||-v<l> P ≅ Q | VΓN | VP])
+    (VPz := substS nN VP (zeroValid VΓ))
+    (VQz := substS nN VQ (zeroValid VΓ))
+    (Vhz : [Γ ||-v<l> hz : P[tZero..] | VΓ | VPz]) 
+    (Vhz' : [Γ ||-v<l> hz' : Q[tZero..] | VΓ | VQz])
+    (Vheqz : [Γ ||-v<l> hz ≅ hz' : P[tZero..] | VΓ | VPz])
+    (VPs := elimSuccHypTyValid (nN := nN) VΓ VP)
+    (VQs := elimSuccHypTyValid (nN := nN) VΓ VQ)
+    (Vhs : [Γ ||-v<l> hs : _ | VΓ | VPs]) 
+    (Vhs' : [Γ ||-v<l> hs' : _ | VΓ | VQs])
+    (Vheqs : [Γ ||-v<l> hs ≅ hs' : _ | VΓ | VPs]) 
+    (Vn : [Γ ||-v<l> n : _ | VΓ | VN])
+    (Vn' : [Γ ||-v<l> n' : _ | VΓ | VN])
+    (Veqn : [Γ ||-v<l> n ≅ n' : _ | VΓ | VN])
+    (VPn := substS nN VP Vn) :
+    [Γ ||-v<l> tNatElim P hz hs n ≅ tNatElim Q hz' hs' n' : _ | VΓ | VPn].
+Proof.
+  constructor; intros.
+  pose (Vuσ := liftSubstS' nN VN Vσ).
+  instValid Vσ; instValid Vuσ; escape.
+  irrelevance0.  1: now rewrite singleSubstComm'.
+  unshelve eapply natElimRedEq; tea; fold subst_term.
+  6-11: irrelevance; now rewrite elimSuccHypTy_subst.
+  3,4: rewrite elimSuccHypTy_subst; eapply validTy; tea; eapply elimSuccHypTyValid.
+  + intros m Rm.
+    rewrite up_single_subst. 
+    unshelve eapply validTy; cycle 1; tea.
+    unshelve econstructor; [now bsimpl| now cbn].
+  + intros m Rm.
+    rewrite up_single_subst. 
+    unshelve eapply validTy; cycle 1; tea.
+    unshelve econstructor; [now bsimpl| now cbn].
+  + intros m m' Rm Rm' Rmm'; cbn.
+    irrelevance0. 1: now rewrite up_single_subst.
+    rewrite up_single_subst.
+    eapply transEq; cycle 1.
+    - unshelve eapply validTyEq. 
+      7: tea. 1: tea.
+      unshelve econstructor; [now bsimpl| now cbn].
+    - unshelve eapply validTyExt; cycle 1 ; tea.
+    1,2: unshelve econstructor; [now bsimpl| now cbn].
+    unshelve econstructor; [|now cbn].
+    bsimpl. eapply reflSubst.
+    Unshelve. 1: tea.
+    eapply validTy; tea.
+    unshelve econstructor; [| now cbn]; now bsimpl.
+Qed.
+
+Lemma elimSuccHypTyCongValid {Γ l nN P P'}
+    (VΓ : [||-v Γ])
+    (VN := natValid (l:=l) VΓ)
+    (VΓN := validSnoc nN VΓ VN)
+    (VP : [Γ ,, vass nN tNat ||-v<l> P | VΓN])
+    (VP' : [Γ ,, vass nN tNat ||-v<l> P' | VΓN])
+    (VeqP : [Γ ,, vass nN tNat ||-v<l> P ≅ P' | VΓN | VP]) :
+    [Γ ||-v<l> elimSuccHypTy nN P ≅ elimSuccHypTy nN P' | VΓ | elimSuccHypTyValid VΓ VP].
+  Proof.
+    unfold elimSuccHypTy.
+    eapply irrelevanceEq.
+    assert [Γ,, vass nN tNat ||-v< l > P'[tSucc (tRel 0)]⇑ | validSnoc nN VΓ VN]. 1:{
+      eapply substLiftS; tea.
+      eapply irrelevanceTm.
+      eapply succValid.
+      eapply irrelevanceTm.
+      change tNat with tNat⟨@wk1 Γ nN tNat⟩ at 2.
+      eapply var0Valid.
+    }
+    eapply PiCong.
+    - eapply simpleArrValid; tea.
+    - eapply reflValidTy.
+    - eapply simpleArrCongValid; tea.
+      eapply substLiftSEq; tea.
+    Unshelve. all: tea.
+    unshelve eapply irrelevanceTm; tea.
+    2: eapply succValid.
+    unshelve eapply irrelevanceTm'.
+    5: unshelve eapply var0Valid; tea.
+    now bsimpl.
+  Qed.
+
+End Nat.
