theories/Substitution/Introductions/SimpleArr.v
@@ -1,0 +1,64 @@
+From LogRel.AutoSubst Require Import core unscoped Ast Extra.
+From LogRel Require Import Utils BasicAst Notations Context NormalForms Weakening
+  DeclarativeTyping GenericTyping LogicalRelation Validity.
+From LogRel.LogicalRelation Require Import Escape Reflexivity Neutral Weakening Irrelevance.
+From LogRel.Substitution Require Import Irrelevance Properties.
+From LogRel.Substitution.Introductions Require Import Universe Pi Application.
+
+Set Universe Polymorphism.
+
+Section SimpleArrValidity.
+
+  Context `{GenericTypingProperties}.
+
+  Lemma simpleArrValid {l Γ F G} (VΓ : [||-v Γ])
+    (VF : [Γ ||-v< l > F | VΓ ])
+    (VG : [Γ ||-v< l > G | VΓ]) : 
+    [Γ ||-v<l> arr F G | VΓ].
+  Proof.
+    unshelve eapply PiValid; tea.
+    replace G⟨↑⟩ with G⟨@wk1 Γ anDummy F⟩ by now bsimpl.
+    now eapply wk1ValidTy.
+  Qed.
+
+  Lemma simpleArrCongValid {l Γ F F' G G'} (VΓ : [||-v Γ])
+    (VF : [Γ ||-v< l > F | VΓ ])
+    (VF' : [Γ ||-v< l > F' | VΓ ])
+    (VeqF : [Γ ||-v< l > F ≅ F' | VΓ | VF])
+    (VG : [Γ ||-v< l > G | VΓ ])
+    (VG' : [Γ ||-v< l > G' | VΓ ])
+    (VeqG : [Γ ||-v< l > G ≅ G' | VΓ | VG]) : 
+    [Γ ||-v<l> arr F G ≅ arr F' G' | VΓ | simpleArrValid _ VF VG].
+  Proof.
+    eapply irrelevanceEq.
+    unshelve eapply PiCong; tea. 
+    + replace G⟨↑⟩ with G⟨@wk1 Γ anDummy F⟩ by now bsimpl.
+      now eapply wk1ValidTy.
+    + replace G'⟨↑⟩ with G'⟨@wk1 Γ anDummy F'⟩ by now bsimpl.
+      now eapply wk1ValidTy.
+    + replace G'⟨↑⟩ with G'⟨@wk1 Γ anDummy F⟩ by now bsimpl.
+      eapply irrelevanceEq'.
+      2: now eapply wk1ValidTyEq.
+      now bsimpl.
+    Unshelve. 2: tea.
+  Qed.
+
+  Lemma simple_appValid {Γ t u F G l}
+    (VΓ : [||-v Γ])
+    {VF : [Γ ||-v<l> F | VΓ]}
+    (VG : [Γ ||-v<l> G | VΓ]) 
+    (VΠ : [Γ ||-v<l> arr F G | VΓ])
+    (Vt : [Γ ||-v<l> t : arr F G | _ | VΠ])
+    (Vu : [Γ ||-v<l> u : F | _ | VF]) :
+    [Γ ||-v<l> tApp t u : G| _ | VG].
+  Proof.
+    eapply irrelevanceTm'.
+    2: eapply appValid; tea.
+    now bsimpl.
+  Unshelve. all: tea.
+  Qed.
+
+
+End SimpleArrValidity.
+
+
