theories/Substitution/Introductions/Var.v
@@ -1,0 +1,22 @@
+(** * LogRel.Introductions.Var : Validity of variables. *)
+From LogRel.AutoSubst Require Import core unscoped Ast Extra.
+From LogRel Require Import Utils BasicAst Notations Context NormalForms Weakening
+  DeclarativeTyping DeclarativeInstance GenericTyping LogicalRelation Validity.
+From LogRel.LogicalRelation Require Import Escape Irrelevance Reflexivity Transitivity Universe Weakening Neutral Induction NormalRed.
+From LogRel.Substitution Require Import Irrelevance Properties Conversion Reflexivity SingleSubst Escape.
+
+Set Universe Polymorphism.
+Set Printing Primitive Projection Parameters.
+
+Section Var.
+  Context `{GenericTypingProperties}.
+  
+  Lemma var0Valid {Γ l nA A} (VΓ : [||-v Γ]) (VA : [Γ ||-v<l> A | VΓ]) :
+    [Γ,, vass nA A ||-v<l> tRel 0 : _ | validSnoc nA VΓ VA | wk1ValidTy nA _ VA ].
+  Proof.
+    constructor; intros; cbn.
+    + epose (validHead Vσ); irrelevance.
+    + epose (eqHead Vσσ'); irrelevance.
+  Qed.
+  
+End Var.
